coq/Wt.v
@@ -1,0 +1,303 @@
+Require Import BitsToLists.
+Require Import TypeInference.
+
+Fixpoint size_uaction
+  {pos_t var_t fn_name_t reg_t ext_fn_t: Type}
+  (ua: Syntax.uaction pos_t var_t fn_name_t reg_t ext_fn_t) {struct ua}
+: nat :=
+  match ua  with
+  | UError err => 0
+  | UFail tau => 0
+  | UVar var => 0
+  | UConst cst => 0
+  | UAssign v ex => 1 + size_uaction ex
+  | USeq a1 a2 => 1 + size_uaction a1 + size_uaction a2
+  | UBind v ex body => 1 + size_uaction ex + size_uaction body
+  | UIf cond tbranch fbranch =>
+    1 + size_uaction cond + size_uaction tbranch + size_uaction fbranch
+  | URead port idx => 0
+  | UWrite port idx value => 1 + size_uaction value
+  | UUnop ufn1 arg1 => 1 + size_uaction arg1
+  | UBinop ufn2 arg1 arg2 => 1 + size_uaction arg1 + size_uaction arg2
+  | UExternalCall ufn arg => 1 + size_uaction arg
+  | UInternalCall ufn args =>
+    1 + size_uaction (int_body ufn) + list_sum (map size_uaction args)
+  | UAPos p e => 1 + size_uaction e
+  | USugar s => 1 + size_sugar s
+  end
+with size_sugar
+  {pos_t var_t fn_name_t reg_t ext_fn_t: Type}
+  (s: usugar pos_t var_t fn_name_t reg_t ext_fn_t) {struct s}
+: nat :=
+   match s with
+   | UErrorInAst => 0
+   | USkip => 0
+   | UConstBits _ => 0
+   | UConstString _ => 0
+   | UConstEnum _ _ => 0
+   | UProgn l => 1 + list_sum (map size_uaction l)
+   | ULet bindings body =>
+     1 + size_uaction body
+     + list_sum (map (fun '(_, a) => size_uaction a) bindings)
+   | UWhen cond body => size_uaction cond + size_uaction body
+   | USwitch cond default branches =>
+     1 + size_uaction cond + size_uaction default
+     + list_sum
+       (map (fun '(a,b) => S (size_uaction a + size_uaction b)) branches)
+   | UStructInit sig l => 1 + list_sum (map (fun '(_, a) => size_uaction a) l)
+   | UArrayInit tay l => 1 + list_sum (map size_uaction l)
+   | UCallModule fR fSigma fn args =>
+     1 + size_uaction (int_body fn) + list_sum (map size_uaction args)
+   end.
+
+Section WT.
+  Variables pos_t fn_name_t: Type.
+  Variable var_t: Type.
+  Context {eq_dec_var_t: EqDec var_t}.
+  Variable ext_fn_t: Type.
+  Variable reg_t: Type.
+  Variable R : reg_t -> type.
+  Variable Sigma: ext_fn_t -> ExternalSignature.
+
+
+  Lemma cast_action'_eq:
+    forall
+      (p: pos_t) (sig: tsig var_t) (tau1 tau2: type)
+      (a: TypedSyntax.action pos_t var_t fn_name_t R Sigma sig tau1)
+      (e: error_message var_t fn_name_t) a',
+    TypeInference.cast_action' R Sigma p tau2 a e = Success a' ->
+    exists p : tau1 = tau2, a' = eq_rect _ _ a _ p.
+  Proof.
+    unfold TypeInference.cast_action'. intros.
+    destr_in H. subst.
+    unfold eq_rect_r in H. simpl in H. inv H.
+    exists eq_refl; reflexivity. inv H.
+  Qed.
+
+  Lemma cast_action_eq:
+    forall
+      (p: pos_t) (sig: tsig var_t) (tau1 tau2: type)
+      (a: TypedSyntax.action pos_t var_t fn_name_t R Sigma sig tau1) a',
+    TypeInference.cast_action R Sigma p tau2 a = Success a'
+    -> exists p : tau1 = tau2, a' = eq_rect _ _ a _ p.
+  Proof.
+    intros. unfold TypeInference.cast_action in H.
+    eapply cast_action'_eq; eauto.
+  Qed.
+
+  Lemma type_action_wt:
+    forall ua p sig a,
+      type_action R Sigma p sig ua = Success a ->
+      wt_action pos_t fn_name_t var_t ext_fn_t reg_t R Sigma sig ua (projT1 a).
+  Proof.
+    intros ua.
+    remember (size_uaction ua).
+    revert ua Heqn.
+    pattern n.
+    eapply Nat.strong_right_induction with (z:=0).
+    { red. red. intros. subst. tauto. } 2: lia.
+    intros n0 _ Plt ua Heqn. subst.
+    assert (Plt':
+              forall
+                (ua': Syntax.uaction pos_t var_t fn_name_t reg_t ext_fn_t),
+                size_uaction ua' < size_uaction ua ->
+                forall (p : pos_t) (sig : tsig var_t)
+                       (a : {tau : type & TypedSyntax.action pos_t var_t fn_name_t R Sigma sig tau}),
+                  type_action R Sigma p sig ua' = Success a ->
+                  wt_action pos_t fn_name_t var_t ext_fn_t reg_t R Sigma sig ua' (projT1 a)
+           ).
+    { intros. eapply Plt. 3: reflexivity. lia. auto. eauto. } clear Plt.
+    rename Plt' into IHua. clear n.
+    destruct ua; simpl; intros.
+    - inv H.
+    - inv H. simpl. constructor.
+    - destr_in H; inv H.
+      unfold opt_result in Heqr.
+      destr_in Heqr; inv Heqr. simpl.
+      econstructor. econstructor; eauto.
+    - inv H. simpl. econstructor.
+    - repeat destr_in H; inv H. simpl. econstructor.
+      eapply IHua. simpl. lia. eauto.
+      unfold opt_result in Heqr. destr_in Heqr; inv Heqr.
+      edestruct cast_action_eq. eauto. simpl in H. rewrite x.
+      econstructor; eauto.
+    - repeat destr_in H; inv H. simpl. econstructor.
+      eapply IHua. simpl. lia. eauto.
+      eapply IHua. simpl. lia. eauto.
+    - repeat destr_in H; inv H. simpl. econstructor.
+      eapply IHua. simpl. lia. eauto.
+      eapply IHua. simpl. lia. eauto.
+    - repeat destr_in H; inv H. simpl. econstructor.
+      eapply cast_action_eq in Heqr0. destruct Heqr0. rewrite <- x.
+      eapply IHua. simpl. lia. eauto.
+      eapply IHua. simpl. lia. eauto.
+      eapply cast_action_eq in Heqr3. destruct Heqr3. rewrite <- x.
+      eapply IHua. simpl. lia. eauto.
+    - repeat destr_in H; inv H. simpl. econstructor.
+    - repeat destr_in H; inv H. simpl. econstructor.
+      eapply cast_action_eq in Heqr0. destruct Heqr0. rewrite <- x.
+      eapply IHua. simpl. lia. eauto.
+    - repeat destr_in H; inv H. simpl.
+      eapply IHua in Heqr. 2: simpl; lia. simpl in *.
+      eapply cast_action_eq in Heqr1. destruct Heqr1. subst.
+      destruct ufn1; simpl in *.
+      + repeat destr_in Heqr0; simpl in Heqr0; inv Heqr0.
+        destr_in Heqr1; inv Heqr1. simpl in *. econstructor. eauto.
+        simpl in *. econstructor. eauto.
+      + repeat destr_in Heqr0; simpl in Heqr0; inv Heqr0; simpl in *.
+        econstructor. eauto.
+        econstructor. rewrite <- x; eauto.
+        econstructor. eauto.
+      + repeat destr_in Heqr0; simpl in Heqr0; inv Heqr0; simpl in *;
+          repeat destr_in Heqr1; inv Heqr1; simpl in *.
+        econstructor. eauto.
+        econstructor. eauto.
+        econstructor. eauto.
+        econstructor. eauto.
+        econstructor. eauto.
+        econstructor. eauto.
+      + repeat destr_in Heqr0; simpl in Heqr0; inv Heqr0; simpl in *;
+          repeat destr_in Heqr1; inv Heqr1; simpl in *.
+        econstructor. eauto. eauto.
+        econstructor. rewrite x in Heqr; simpl in Heqr. eauto. eauto.
+      + repeat destr_in Heqr0; simpl in Heqr0; inv Heqr0; simpl in *;
+          repeat destr_in Heqr1; inv Heqr1; simpl in *.
+        econstructor. eauto.
+        econstructor. rewrite x in Heqr; simpl in Heqr. eauto.
+    - repeat destr_in H; inv H. simpl.
+      eapply IHua in Heqr. 2: simpl; lia. simpl in *.
+      eapply IHua in Heqr0. 2: simpl; lia. simpl in *.
+      eapply cast_action_eq in Heqr2. destruct Heqr2. subst.
+      eapply cast_action_eq in Heqr3. destruct Heqr3. subst.
+      destruct s, s0; simpl in *. subst.
+      destruct ufn2; simpl in *.
+      + inv Heqr1. simpl. econstructor; eauto.
+        replace (arg1Sig (PrimSignatures.Sigma2 s1)) with (arg2Sig (PrimSignatures.Sigma2 s1)). eauto.
+        rewrite <- H0. simpl. eauto.
+      + repeat destr_in Heqr1; simpl in *; inv Heqr1; simpl in *; try (econstructor; eauto; fail).
+        * replace (s0 + s) with (s + s0). econstructor; eauto. lia.
+      + repeat destr_in Heqr1; simpl in *; inv Heqr1; simpl in *; try (econstructor; eauto; fail).
+      + repeat destr_in Heqr1; simpl in *; inv Heqr1; simpl in *; try (econstructor; eauto; fail).
+    - repeat destr_in H; inv H. simpl.
+      econstructor.
+      eapply cast_action_eq in Heqr0. destruct Heqr0. subst. rewrite <- x; eauto.
+    - repeat destr_in H; inv H. simpl.
+      eapply cast_action_eq in Heqr2. destruct Heqr2. subst.
+      eapply IHua in Heqr1. 2: simpl; lia.
+      econstructor. 2: rewrite <- x; eauto.
+
+      unfold assert_argtypes in Heqr0.
+
+      Lemma assert_argtypes'_same_length:
+        forall {T} sig p (src: T) nexpected fn_name l1 l2 s0,
+          assert_argtypes'
+            (sig:=sig)
+            (fn_name_t := fn_name_t)
+            (pos_t := pos_t)
+            (var_t := var_t)
+            R Sigma src nexpected fn_name p l1 l2 = Success s0 ->
+          List.length l1 = List.length l2.
+      Proof.
+        induction l1; simpl; intros; eauto.
+        - destr_in H; inv H. reflexivity.
+        - repeat destr_in H; inv H. simpl.
+          eapply IHl1 in Heqr0. rewrite Heqr0; reflexivity.
+      Qed.
+
+      Lemma argtypes_app:
+        forall {T} sig p (src: T) nexpected fn_name l1 l2 l3 l4 s0,
+          assert_argtypes'
+            (sig:=sig)
+            (fn_name_t := fn_name_t)
+            (pos_t := pos_t)
+            (var_t := var_t)
+            R Sigma src nexpected fn_name p
+                           (l1 ++ l2)
+                           (l3 ++ l4) =
+          Success s0 ->
+          List.length l1 = List.length l3 ->
+          List.length l2 = List.length l4 ->
+          exists s1 s2,
+            assert_argtypes' R Sigma src nexpected fn_name p l1 l3 = Success s1 /\
+            assert_argtypes' R Sigma src nexpected fn_name p l2 l4 = Success s2.
+      Proof.
+        induction l1; simpl; intros; eauto.
+        - destruct l3; simpl in *; try lia.
+          eexists; eexists; split; eauto.
+        - destruct l3; simpl in *; try lia.
+          repeat destr_in H; inv H.
+          eapply IHl1 in Heqr0; try lia.
+          destruct Heqr0 as (s3 & s4 & EQ1 & EQ2).
+          rewrite EQ1, EQ2.
+          eexists; eexists; split; eauto.
+      Qed.
+
+      Lemma argtypes_ok:
+        forall {T} args sig p s (src: T) nexpected fn_name argspec argpos s0
+               (IHua:
+               forall ua' : uaction pos_t var_t fn_name_t reg_t ext_fn_t,
+                 In ua' args ->
+                 forall (p : pos_t) (sig : tsig var_t)
+                        (a : {tau : type & TypedSyntax.action pos_t var_t fn_name_t R Sigma sig tau}),
+                   type_action R Sigma p sig ua' = Success a ->
+                   wt_action pos_t fn_name_t var_t ext_fn_t reg_t R Sigma sig ua' (projT1 a)
+               )
+               (SAMELEN:           List.length argpos = List.length s)
+        ,
+          result_list_map (type_action R Sigma p sig) args = Success s ->
+          assert_argtypes' R Sigma src nexpected fn_name p
+                           (rev argspec)
+                           (rev (combine argpos s)) =
+          Success s0 ->
+          Forall2 (wt_action pos_t fn_name_t var_t ext_fn_t reg_t R Sigma sig) args (map snd argspec).
+      Proof.
+        induction args; simpl; intros; eauto.
+        - inv H. simpl in H0.
+          apply assert_argtypes'_same_length in H0. rewrite combine_nil in H0. simpl in H0.
+          rewrite rev_length in H0.
+          apply length_zero_iff_nil in H0. subst. simpl. constructor.
+        - assert ( List.length (rev argspec) = List.length (rev (combine argpos s))).
+          apply assert_argtypes'_same_length in H0. auto.
+          repeat destr_in H; inv H. simpl in H1.
+          simpl in SAMELEN. destruct argpos; simpl in SAMELEN; try lia.
+          simpl in H1. rewrite app_length in H1. simpl in H1.
+          destruct argspec; simpl in H1; try lia. simpl.
+          simpl in H0.
+          edestruct @argtypes_app as (s3 & s4 & EQ1 & EQ2). apply H0.
+          rewrite app_length in H1. simpl in H1. lia. reflexivity.
+          constructor.
+          simpl in EQ2. repeat destr_in EQ2; inv EQ2. simpl.
+          eapply IHua in Heqr; eauto.
+          apply cast_action_eq in Heqr1. destruct Heqr1. rewrite <- x; auto.
+          eapply IHargs. intros; eapply IHua; eauto.
+          2: apply Heqr0. inv SAMELEN. reflexivity. eauto.
+      Qed.
+
+      eapply argtypes_ok.
+      4: apply Heqr0.
+      3: eauto.
+      {
+        intros; eapply IHua; eauto. simpl.
+        cut (size_uaction ua' <= list_sum (map size_uaction args)). lia.
+        clear - H. revert ua' args H. induction args; simpl; intros; eauto. easy.
+        destruct H. subst. lia.
+        apply IHargs in H. lia.
+      }
+      rewrite map_length.
+
+      Lemma result_list_map_length:
+        forall {A B F} (f: A -> result B F) l l',
+          result_list_map f l = Success l' ->
+          List.length l' = List.length l.
+      Proof.
+        induction l; simpl; intros; eauto.
+        inv H; reflexivity.
+        repeat destr_in H; inv H. simpl.
+        erewrite IHl; eauto.
+      Qed.
+      erewrite <- result_list_map_length; eauto.
+    - repeat destr_in H; inv H. simpl. constructor.  eapply IHua; eauto.
+    - inv H.
+  Qed.
+
+End WT.
